src/proof/get.v
@@ -17,13 +17,13 @@ Context `{!mapG Σ KKey.t PureKObject.t}.
 Context `{!mapG Σ KKey.t (gset KKey.t)}.
 Context `{!auth_setG Σ KKey.t}.
 
-Lemma wp_objGet_replicaset_ptsto_mut key γ_state γ_children γ_fresh_keys pure_rs:
+Lemma wp_State__objGet_replicaset l key γ_state γ_children γ_fresh_keys pure_rs:
   {{{ is_pkg_init apimodel ∗
-      "#Hinv" ∷ is_kubernetes_state γ_state γ_children γ_fresh_keys ∗
+      "#Hisk" ∷ is_kubernetes γ_state γ_children γ_fresh_keys l ∗
       "%Hkind_eq" ∷ ⌜ KKey.Kind' key = "ReplicaSet"%go ⌝ ∗
       "Hown_rs" ∷ key [[ γ_state ]]↦ (PureKObject.ReplicaSet pure_rs)
   }}}
-    @! apimodel.objGet #key
+    l @ (ptrT.id apimodel.State.id) @ "objGet" #key
   {{{ ptr rs, RET (#(interface.mk (ptrT.id v1.ReplicaSet.id) #ptr), #true);
       PureReplicaSet.deepown_l ptr rs pure_rs 1 ∗
       ⌜ PureReplicaSet.well_formed pure_rs ⌝ ∗
@@ -32,10 +32,9 @@ Lemma wp_objGet_replicaset_ptsto_mut key γ_state γ_children γ_fresh_keys pure
       key [[ γ_state ]]↦ (PureKObject.ReplicaSet pure_rs)
   }}}.
 Proof.
-  wp_start as "H". iNamed "H".
+  wp_start as "H". iNamed "H". iNamed "Hisk".
   wp_apply wp_with_defer. iIntros (defer) "Hdefer". simpl subst. wp_auto.
-  wp_apply wp_globals_get. wp_apply wp_Mutex__Lock; [done|]. iIntros "[Hown_Mutex H]". iNamedPrefix "H" "Hinv_". wp_auto.
-  wp_apply wp_globals_get. wp_apply wp_globals_get.
+  wp_apply wp_Mutex__Lock; [done|]. iIntros "[Hown_Mutex H]". iNamedPrefix "H" "Hinv_". wp_auto.
   iAssert (⌜ abs_state !! key = Some (PureKObject.ReplicaSet pure_rs) ⌝%I) with "[Hown_rs Hinv_Hown_abs]" as "%Hkey_in_abs".
   { iDestruct (map_valid with "Hinv_Hown_abs Hown_rs") as %Hlookup.
     iPureIntro; exact Hlookup. }
@@ -59,18 +58,18 @@ Proof.
   { destruct Hinv_Hghost_well_formed. apply Habs_state_well_formed. exact Hkey_in_abs. }
   destruct Hagree as [Hkind [Hnamespace Hname]].
   iCombineNamed "Hinv_*" as "H".
-  wp_apply (wp_Mutex__Unlock _ (is_kubernetes_state_inner γ_state γ_children γ_fresh_keys)
+  wp_apply (wp_Mutex__Unlock _ (kubernetes_inv γ_state γ_children γ_fresh_keys l)
   with "[$Hown_Mutex H]").
   { iNamed "H". iFrame. iFrame "#". done. }
   iApply "HΦ". iFrame. done.
 Qed.
 
-Lemma wp_ReplicaSetMutGet_ptsto_mut namespace name γ_state γ_children γ_fresh_keys pure_rs:
+Lemma wp_State__ReplicaSetMutGet l namespace name γ_state γ_children γ_fresh_keys pure_rs:
   {{{ is_pkg_init apimodel ∗
-      "#Hinv" ∷ is_kubernetes_state γ_state γ_children γ_fresh_keys ∗
+      "#Hisk" ∷ is_kubernetes γ_state γ_children γ_fresh_keys l ∗
       "Hown_rs" ∷ (mk_replicaset_key namespace name) [[ γ_state ]]↦ (PureKObject.ReplicaSet pure_rs)
   }}}
-    @! apimodel.ReplicaSetMutGet #namespace #name
+    l @ (ptrT.id apimodel.State.id) @ "ReplicaSetMutGet" #namespace #name
   {{{ ptr rs, RET (#ptr, #interface.nil);
       PureReplicaSet.deepown_l ptr rs pure_rs 1 ∗
       ⌜ PureReplicaSet.well_formed pure_rs ⌝ ∗
@@ -80,7 +79,7 @@ Lemma wp_ReplicaSetMutGet_ptsto_mut namespace name γ_state γ_children γ_fresh
   }}}.
 Proof.
   wp_start as "H". iNamed "H". wp_auto.
-  wp_apply (wp_objGet_replicaset_ptsto_mut with "[$Hown_rs]"); [iFrame "#"; done|].
+  wp_apply (wp_State__objGet_replicaset with "[$Hown_rs]"); [iFrame "#"; done|].
   iIntros (ptr rs) "(Hdeepown_l_rs & %Hwell_formed_pure_rs & -> & -> & Hown_pure_rs)". wp_auto.
   unshelve wp_apply wp_interface_checked_type_assert; try tc_solve.
   { iPureIntro. intros ptr_id. exists ptr. done. }
@@ -93,12 +92,12 @@ Proof.
   iApply "HΦ". iFrame. done.
 Qed.
 
-Lemma wp_ReplicaSetGet_ptsto_mut namespace name γ_state γ_children γ_fresh_keys pure_rs:
+Lemma wp_State__ReplicaSetGet l namespace name γ_state γ_children γ_fresh_keys pure_rs:
   {{{ is_pkg_init apimodel ∗
-      "#Hinv" ∷ is_kubernetes_state γ_state γ_children γ_fresh_keys ∗
+      "#Hisk" ∷ is_kubernetes γ_state γ_children γ_fresh_keys l ∗
       "Hown_rs" ∷ (mk_replicaset_key namespace name) [[ γ_state ]]↦ (PureKObject.ReplicaSet pure_rs)
   }}}
-    @! apimodel.ReplicaSetGet #namespace #name
+    l @ (ptrT.id apimodel.State.id) @ "ReplicaSetGet" #namespace #name
   {{{ ptr rs dq, RET (#ptr, #interface.nil);
       PureReplicaSet.deepown_l ptr rs pure_rs dq ∗
       ⌜ PureReplicaSet.well_formed pure_rs ⌝ ∗
@@ -108,8 +107,8 @@ Lemma wp_ReplicaSetGet_ptsto_mut namespace name γ_state γ_children γ_fresh_ke
   }}}.
 Proof.
   wp_start as "H". iNamed "H". wp_auto.
-  wp_apply (wp_ReplicaSetMutGet_ptsto_mut with "[$Hown_rs]"); [done|].
-  iIntros (l rs) "(Hdeepown_l_rs & %Hwell_formed_pure_rs & -> & -> & Hown_rs)". wp_auto.
+  wp_apply (wp_State__ReplicaSetMutGet with "[$Hown_rs]"); [done|].
+  iIntros (ptr rs) "(Hdeepown_l_rs & %Hwell_formed_pure_rs & -> & -> & Hown_rs)". wp_auto.
   iApply "HΦ". iFrame. done.
 Qed.
 
