src/proof/index.v
@@ -18,23 +18,22 @@ Context `{!mapG Σ KKey.t (gset KKey.t)}.
 Context `{!auth_setG Σ KKey.t}.
 
 (* TODO: revisit this spec *)
-Lemma wp_ByIndex_pod_ptsto_mut kind index_name indexed_value
+Lemma wp_State__ByIndex_pod l kind index_name indexed_value
   γ_state γ_children γ_fresh_keys parent_key owned_parent owned_pod_map owned_child_keys:
   {{{ is_pkg_init apimodel ∗
-      "#inv" ∷ is_kubernetes_state γ_state γ_children γ_fresh_keys ∗
-      "own_parent" ∷ parent_key [[ γ_state ]]↦ owned_parent ∗
-      "own_pods" ∷ ([∗ map] key ↦ pod ∈ owned_pod_map, key [[ γ_state ]]↦ PureKObject.Pod pod) ∗
-      "own_child_keys" ∷ parent_key [[ γ_children ]]↦ owned_child_keys ∗
-      "%owned_child_keys_equal_dom_owned_pods" ∷ ⌜ owned_child_keys = dom owned_pod_map ⌝ ∗
-      "%indexed_value" ∷ ⌜ indexed_value = (PureKObject.metadata owned_parent).(PureObjectMeta.UID') ⌝ ∗
-      "%kind" ∷ ⌜ kind = "Pod"%go ⌝ ∗
-      "%index_name" ∷ ⌜ index_name = "podControllerUID"%go ⌝
+      "#Hisk" ∷ is_kubernetes γ_state γ_children γ_fresh_keys l ∗
+      "%Hkind" ∷ ⌜ kind = "Pod"%go ⌝ ∗
+      "%Hindex_name" ∷ ⌜ index_name = "podController"%go ⌝ ∗
+      "%Hindexed_value" ∷ ⌜ indexed_value = (PureKObject.metadata owned_parent).(PureObjectMeta.UID') ⌝ ∗
+      "Hown_parent" ∷ parent_key [[ γ_state ]]↦ owned_parent ∗
+      "Hown_pods" ∷ ([∗ map] key ↦ pod ∈ owned_pod_map, key [[ γ_state ]]↦ PureKObject.Pod pod) ∗
+      "Hown_child_keys" ∷ parent_key [[ γ_children ]]↦ owned_child_keys ∗
+      "%Howned_child_keys_equal_dom_owned_pods" ∷ ⌜ owned_child_keys = dom owned_pod_map ⌝
   }}}
-    @! apimodel.ByIndex #kind #index_name #indexed_value
-  {{{ (l: slice.t) (err: error.t) (objs: list interface.t) (pods: list v1.Pod.t), RET (#l, #err);
-      "l" ∷ l ↦* objs ∗
-      "%err_is_nil" ∷ ⌜ err = interface.nil ⌝ ∗
-      "obj_pts_to_pod" ∷ ([∗ list] obj ; pod ∈ objs ; pods, ∃ (ptr : loc) (owned_pod : PurePod.t),
+    l @ (ptrT.id apimodel.State.id) @ "ByIndex" #kind #index_name #indexed_value
+  {{{ objs_l (objs: list interface.t) (pods: list v1.Pod.t), RET (#objs_l, #interface.nil);
+      "Hobjs_l" ∷ objs_l ↦* objs ∗
+      "Hobj_pts_to_pod" ∷ ([∗ list] obj ; pod ∈ objs ; pods, ∃ (ptr : loc) (owned_pod : PurePod.t),
         ⌜ obj = interface.mk (ptrT.id v1.Pod.id) #ptr ⌝ ∗
         ptr ↦ pod ∗
         PurePod.deepown pod owned_pod 1 ∗
@@ -42,10 +41,10 @@ Lemma wp_ByIndex_pod_ptsto_mut kind index_name indexed_value
         ⌜ obj_has_controller_parent_of (PureKObject.Pod owned_pod) parent_key.(KKey.Kind') parent_key.(KKey.Name') indexed_value ⌝ ∗
         ⌜ PurePod.well_formed owned_pod ⌝
       ) ∗
-      "%key_set_equal_dom_owned_pods" ∷  ⌜ list_to_set (extract_pod_key <$> pods) = dom owned_pod_map ⌝ ∗
-      "own_parent" ∷ parent_key [[ γ_state ]]↦ owned_parent ∗
-      "own_pods" ∷ ([∗ map] key ↦ pod ∈ owned_pod_map, key [[ γ_state ]]↦ PureKObject.Pod pod) ∗
-      "own_child_keys" ∷ parent_key [[ γ_children ]]↦ owned_child_keys
+      "%Hkey_set_equal_dom_owned_pods" ∷  ⌜ list_to_set (extract_pod_key <$> pods) = dom owned_pod_map ⌝ ∗
+      "Hown_parent" ∷ parent_key [[ γ_state ]]↦ owned_parent ∗
+      "Hown_pods" ∷ ([∗ map] key ↦ pod ∈ owned_pod_map, key [[ γ_state ]]↦ PureKObject.Pod pod) ∗
+      "Hown_child_keys" ∷ parent_key [[ γ_children ]]↦ owned_child_keys
   }}}.
 Proof.
 Admitted.
